Dafny/arrays.dfy
@@ -1,0 +1,29 @@
+predicate sorted(a: array<int>)
+  reads a
+{
+  forall j, k :: 0 <= j < k < a.Length ==> a[j] <= a[k]
+}
+
+method binSearch(a:array<int>, K:int) returns (b:bool)
+  requires sorted(a)
+  ensures b == exists i:nat :: i < a.Length && a[i] == K
+{
+  var lo: nat := 0 ;
+  var hi: nat := a.Length ;
+  while (lo < hi)
+    decreases hi - lo
+    invariant  0 <= lo <= hi <= a.Length
+    invariant forall i:nat :: (i < lo || hi <= i < a.Length) ==> a[i] != K
+  {
+    var mid: nat := (lo + hi) / 2 ;
+    if (a[mid] < K) {
+      lo := mid + 1 ;
+    } else if (a[mid] > K) {
+      hi := mid;
+    } else {
+      return true;
+    }
+  }
+  return false ;
+}
+
