Dafny/guide_tutorial.dfy
@@ -1,0 +1,143 @@
+//This is a Dafny program that contains the solutions to the exercises in "Getting Started with Dafny: A Guide".
+
+//Exercise 0 Write a method Max that takes two integer parameters and returns their maximum. Add appropriate annotations and make sure your code verifies.
+
+method Max(a:int,b:int) returns (m:int)
+  ensures m == a <==> a >= b
+  ensures m == b <==> b >= a
+{
+  if (a>=b){
+    m := a;
+  }
+  else{
+    m := b;
+  }
+}
+
+//Exercise 1 Write a test method that calls your Max method from Exercise 0 and then asserts something about the
+
+method TestMax()
+{
+  var res := Max(1,2);
+  assert res == 2;
+}
+
+/* Exercise 2 Using a precondition, change Abs to say it can only be called on negative values.
+Simplify the body of Abs into just one assignment statement and make sure the method still verifies */
+
+method Abs(x:int) returns (y:int)
+  requires x < 0
+  ensures y == -x
+
+{
+  y := -x;
+}
+
+/* Exercise 3 Keeping the postconditions of Abs the same as above, change the body of Abs
+to y := x + 2;. What precondition do you need to annotate the method with in order
+for the verification to go through? And what precondition do you need if the body is
+y := x + 1;? What does that precondition say about calling the method? */
+
+method Abs'(x:int) returns (y:int)
+  requires x == -1
+  ensures y==-x
+{
+  y := x + 2;
+}
+
+/* Exercise 4 Write a function max that returns the larger of two given integer parameters. 
+Write a test method that uses an assert statement to check some property of the value of
+max on some arguments (for example, 34 < max(21,55) or max(21,55) == max(55,21)).*/
+
+function max(a:int,b:int) : int
+  ensures max(a,b) == a ==> a >= b
+  ensures max(a,b) == b ==> b >= a
+{
+  if a >= b then a else b
+}
+
+method TestMax2()
+{
+  assert 34 < max(21,55);
+  assert max(21,55) == max(55,21);
+}
+
+/* Exercise 5 Change the test method in Exercise 4 to put the result of max into a local
+variable and then use an assert statement to check some property of that local variable. 
+Dafny will reject this program, because you’re calling max from real code. Fix this
+problem using a function method.
+*/
+function  max'(a:int,b:int) : int
+{
+  if a >= b then a else b
+}
+
+method TestMax3()
+{
+  var res := max(21,55);
+  assert res == 55;
+  assert res == max(55,21);
+}
+
+/*Exercise 9 The ComputeFib method above is more complicated than necessary. Write
+a simpler program by not introducing a as the Fibonacci number that precedes b, but
+instead introducing a variable c that that succeeds b. Verify that your program is correct.*/
+
+function fib(n: nat): nat
+{
+  if n == 0 then 0
+  else if n == 1 then 1
+  else fib(n - 1) + fib(n - 2)
+}
+
+method ComputeFib(n: nat) returns (b: nat)
+  ensures b == fib(n)
+{
+  if (n == 0) { return 0; }
+  var i := 1;
+  var a := 0;
+  b := 1;
+  while (i < n)
+    invariant 0 < i <= n
+    invariant a == fib(i - 1)
+    invariant b == fib(i)
+  {
+    a, b := b, a + b;
+    i := i + 1;
+  }
+}
+
+/*Exercise 12 Write a method that takes an integer array, which it requires to have at least
+one element, and returns an index to the maximum of the array’s elements. Annotate the
+method with pre- and postconditions that state the intent of the method, and annotate its
+body with loop invariants to verify it.
+*/
+method MaxArray(l:array<int>) returns (m:int)
+  requires l.Length > 0
+  ensures 0 <= m < l.Length
+  ensures forall i :: 0 <= i < l.Length ==> l[m] >= l[i]
+{
+  m := 0;
+  var i := 1;
+  while (i < l.Length)
+    invariant 0 <= i <= l.Length
+    invariant 0 <= m < l.Length
+    invariant forall j :: 0 <= j < i ==> l[m] >= l[j]
+    decreases l.Length - i
+  {
+    if l[i] > l[m]{
+      m := i;
+    }
+    i := i + 1;
+  }
+}
+
+/*Exercise 13 To get practice with quantifiers, modify the definition of function sorted so
+that it returns true only when the array is sorted and all its elements are distinct.*/
+function sorted'(a: array<int>) : bool
+  requires a.Length > 0
+  reads a
+{
+  (forall j, k :: 0 <= j < k < a.Length ==> a[j] <= a[k]) && (forall j, k :: 0 <= j < k < a.Length ==> a[j] != a[k])
+}
+
